Prove step delay

pancake/proofs/ffiTimeScript.sml
@@ -19,23 +19,22 @@ Overload k2mw = “multiword$k2mw”
 
 
 Definition get_bytes_def:
-  get_bytes (:'a) n =
+  get_bytes (:'a) be w =
   let m  = dimindex (:'a) DIV 8;
-      as = GENLIST (λm. (n2w m): 'a word) m;
-      w  = (n2w n):'a word
+      as = GENLIST (λm. (n2w m): 'a word) m
   in
-    MAP (λa. get_byte a w F) as
+    MAP (λa. get_byte a w be) as
 End
 
 
-Definition ntime_input_def:
-  ntime_input (:'a) (f:num -> num # bool) =
+Definition time_input_def:
+  time_input (:'a) be (f:num -> num # bool) =
   let
-    t = FST (f 0);
-    b = if SND (f 0) then 0 else 1
+    t = n2w (FST (f 0)):'a word;
+    b = if SND (f 0) then 0w else (1w:'a word)
   in
-    get_bytes (:'a) t ++
-    get_bytes (:'a) b
+    get_bytes (:'a) be t ++
+    get_bytes (:'a) be b
 End
 
 Definition next_ffi_def:
@@ -45,24 +44,15 @@ End
 
 
 Definition build_ffi_def:
-  build_ffi (:'a) (seq:time_input) io =
+  build_ffi (:'a) be (seq:time_input) io =
      <| oracle    :=
         (λs f conf bytes.
           if s = "get_ffi"
-          then Oracle_return (next_ffi f) (ntime_input (:'a) f)
+          then Oracle_return (next_ffi f) (time_input (:'a) be f)
           else Oracle_final FFI_failed)
       ; ffi_state := seq
       ; io_events := io|> : time_input_ffi
 End
-
-
-(*
-Definition ntime_input_def:
-  ntime_input (f:num -> num # bool) n =
-    ((k2mw (n-1) (FST (f 0))):word8 list) ++
-    [if SND (f 0) then 0w else 1w]
-End
-*)
 
 (*
 [IO_event "get_ffi" []
